extraction: Improve the compilation logic
In particular, be more discriminate about cases in which transitivity
rules get applied.

src/CertifiedExtraction/ADTExamples.v
@@ -18,56 +18,60 @@ Definition MyEnvLists :=
 Example other_test_with_adt'' :
     sigT (fun prog => forall seq, {{ [["arg1" <-- ADT seq as _ ]] :: Nil }}
                             prog
-                          {{ [["ret" <-- SCA _ (List.fold_left (@Word.wplus 32) seq (Word.wordToNat 0)) as _]] :: Nil }} ∪ {{ StringMap.empty _ }} // MyEnvLists).
+                          {{ [["ret" <-- SCA _ (List.fold_left (@Word.wminus 32) seq 0) as _]] :: Nil }} ∪ {{ StringMap.empty _ }} // MyEnvLists).
 Proof.
   econstructor; intros.
-
-  let vhead := gensym "head" in
-  let vtest := gensym "test" in
-  apply (FacadeLoops.CompileLoop (vhead := vhead) (vtest := vtest)); try compile_do_side_conditions.
-  compile_step.
-  intros.
-
-  Lemma ProgOk_Transitivity_Cons_B :
-    forall {av} env ext t1 t1' t2 prog1 prog2 k (v: Comp (Value av)),
-      {{ t1 }}                            prog1     {{ [[Some k <~~ v as kk]] :: t1' kk }}     ∪ {{ ext }} // env ->
-      {{ [[Some k <~~ v as kk]] :: t1' kk }} prog2     {{ [[Some k <~~ v as kk]] :: t2 kk }} ∪ {{ ext }} // env ->
-      {{ t1 }}                      Seq prog1 prog2 {{ [[Some k <~~ v as kk]] :: t2 kk }} ∪ {{ ext }} // env.
-  Proof.
-    eauto using CompileSeq.
-  Qed.
-
-  (* This is a well-behaved version of ProgOk_Transitivity_Cons, but it is not
-     very useful, as the side goal that it creates are in a form in which one
-     would want to apply transitivity again. *)
-  Lemma ProgOk_Transitivity_Cons_Drop :
-    forall {av} env ext t1 t2 prog1 prog2 k (v: Comp (Value av)),
-      {{ t1 }}                     prog1      {{ [[Some k <~~ v as _]]::(DropName k t1) }}     ∪ {{ ext }} // env ->
-      {{ [[Some k <~~ v as _]]::(DropName k t1) }}      prog2      {{ [[Some k <~~ v as kk]]::t2 kk }} ∪ {{ ext }} // env ->
-      {{ t1 }}                Seq prog1 prog2 {{ [[Some k <~~ v as kk]]::t2 kk }} ∪ {{ ext }} // env.
-  Proof.
-    SameValues_Facade_t.
-  Qed.
-
-  (* eapply ProgOk_Transitivity_Cons_B. *)
-  (* rewrite TelEq_swap; try compile_do_side_conditions. *)
-  (* apply CompileSkip. *)
-  (* compile_step. *)
-  (* compile_step. *)
-  
-  compile_step.
-
-  repeat compile_step.
-
-  subst.
-
-  let fop := translate_op Word.wplus in
+  repeat (compile_step || compile_loop).
+  let fop := translate_op Word.wminus in
   apply (CompileBinopOrTest_right_inPlace fop); compile_do_side_conditions.
 Defined.
 
-Print Assumptions other_test_with_adt''.
+Print Assumptions other_test_with_adt''. (* FIXME *)
+
+Opaque Word.wordToNat.
+Opaque Word.natToWord.
+
+Eval compute in (extract_facade other_test_with_adt'').
 
 Eval cbv beta iota zeta delta [extract_facade Fold proj1_sig sig_of_sigT other_test_with_adt'' WrapOpInExpr] in (extract_facade other_test_with_adt'').
+
+Definition fold_comp {TAcc TElem} (f: TAcc -> TElem -> Comp TAcc) seq init :=
+  List.fold_left (fun acc elem =>
+                    ( acc <- acc;
+                      f acc elem )%comp)
+                 seq (ret init).
+
+Example other_test_with_adt''' `{FacadeWrapper (Value (list W)) (list W)} f:
+    sigT (fun prog => {{ Nil }}
+                     prog
+                   {{ [[`"ret" <~~  ( seq <- {s: list W | True };
+                                    res <- fold_comp f seq (Word.natToWord 32 0: W);
+                                    ret (SCA _ res)) as _]] :: Nil }} ∪ {{ StringMap.empty _ }} // MyEnvLists).
+Proof.
+  econstructor; intros.
+
+  rewrite SameValues_Fiat_Bind_TelEq_Generic.
+  (* eapply ProgOk_Transitivity_Cons. *)
+  (* eapply ProgOk_Transitivity_Name. *)
+  eapply ProgOk_Transitivity_Name' with "seq".
+
+  Focus 2.
+  unfold WrappedCons, WrapCons_Generic.
+  unfold WrapComp_Generic at 2.
+
+    Require Import QueryStructure.Specification.Operations.FlattenCompLis.
+  Check flatten_CompList.
+
+
+  unfold WrappedCons, WrapCons_Generic.
+
+  compile_step.
+
+  repeat (compile_step || compile_loop).
+  let fop := translate_op Word.wminus in
+  apply (CompileBinopOrTest_right_inPlace fop); compile_do_side_conditions.
+Defined.
+
 
 Example other_test_with_adt'' :
     sigT (fun prog => forall seq seq', {{ [["arg1" <-- ADT seq as _ ]] :: [["arg2" <--  ADT seq' as _]] :: Nil }}
@@ -102,3 +106,25 @@ Proof.
   Fail fail.
 Abort.
 
+
+
+  Lemma ProgOk_Transitivity_Cons_B :
+    forall {av} env ext t1 t1' t2 prog1 prog2 k (v: Comp (Value av)),
+      {{ t1 }}                            prog1     {{ [[Some k <~~ v as kk]] :: t1' kk }}     ∪ {{ ext }} // env ->
+      {{ [[Some k <~~ v as kk]] :: t1' kk }} prog2     {{ [[Some k <~~ v as kk]] :: t2 kk }} ∪ {{ ext }} // env ->
+      {{ t1 }}                      Seq prog1 prog2 {{ [[Some k <~~ v as kk]] :: t2 kk }} ∪ {{ ext }} // env.
+  Proof.
+    eauto using CompileSeq.
+  Qed.
+
+  (* This is a well-behaved version of ProgOk_Transitivity_Cons, but it is not
+     very useful, as the side goal that it creates are in a form in which one
+     would want to apply transitivity again. *)
+  Lemma ProgOk_Transitivity_Cons_Drop :
+    forall {av} env ext t1 t2 prog1 prog2 k (v: Comp (Value av)),
+      {{ t1 }}                     prog1      {{ [[Some k <~~ v as _]]::(DropName k t1) }}     ∪ {{ ext }} // env ->
+      {{ [[Some k <~~ v as _]]::(DropName k t1) }}      prog2      {{ [[Some k <~~ v as kk]]::t2 kk }} ∪ {{ ext }} // env ->
+      {{ t1 }}                Seq prog1 prog2 {{ [[Some k <~~ v as kk]]::t2 kk }} ∪ {{ ext }} // env.
+  Proof.
+    SameValues_Facade_t.
+  Qed.
