src/CertifiedExtraction/Extraction/External/External.v
@@ -1,7 +1,8 @@
 Require Export
-        CertifiedExtraction.Extraction.External.FacadeADTs
         CertifiedExtraction.Extraction.External.ScalarMethods
         CertifiedExtraction.Extraction.External.GenericMethods
         CertifiedExtraction.Extraction.External.GenericADTMethods
         CertifiedExtraction.Extraction.External.GenericADTTactics
-        CertifiedExtraction.Extraction.External.ScalarMethodTactics.
+        CertifiedExtraction.Extraction.External.ScalarMethodTactics
+        CertifiedExtraction.Extraction.External.FacadeADTs
+        CertifiedExtraction.Extraction.External.LoopTactics.
