src/CertifiedExtraction/Extraction/Extraction.v
@@ -9,65 +9,9 @@ Require Import
 
 Global Open Scope string_scope.
 
-Ltac compile_simple_internal env cmp ext :=
-  match cmp with
-  | ret (SCA ?av (?op ?lhs ?rhs)) => let facade_op := translate_op op in compile_binop av facade_op lhs rhs ext
-  | ret (@bool2val ?av (?op ?lhs ?rhs)) => let facade_op := translate_op op in compile_binop av facade_op lhs rhs ext
-  | ret (@bool2val ?av (@dec2bool _ _ (?op ?lhs ?rhs))) => let facade_op := translate_op op in compile_binop av facade_op lhs rhs ext
-  | ret (SCA _ ?w) => compile_constant w; compile_do_side_conditions
-  | ret (SCA ?av ?w) => compile_read (SCA av w) ext; compile_do_side_conditions
-  | ret (SCA ?av (?f ?w)) => compile_external_call_SCA av env f w ext
-  | (if ?t then ?tp else ?fp) => compile_if t tp fp
-  end.
-
-Hint Rewrite WrapComp_W_rewrite : compile_simple_db.
-
-Ltac compile_simple name cmp :=
-  debug "Compiling simple pattern";
-  autorewrite with compile_simple_db;  (* Rewrite using user-provided lemmas *)
-  match_ProgOk ltac:(fun prog pre post ext env => (* Recapture cmp after rewriting *)
-                       match constr:(pre, post) with
-                       | (?tenv, Cons ?s ?cmp (fun _ => ?tenv)) => compile_simple_internal env cmp ext
-                       end).
-
-Ltac compile_simple_in_place_internal env cmp cmp' tenv ext :=
-  match cmp' with
-  | (if ?t then ?tp else ?fp) => compile_if_in_place t tp fp
-  | _ => fail "compile_simple_internal can't compile this:" cmp cmp' tenv ext
-  end.
-
-Ltac compile_simple_in_place name cmp cmp' :=
-  debug "Compiling simple pattern";
-  autorewrite with compile_simple_db;  (* Rewrite using user-provided lemmas *)
-  match_ProgOk ltac:(fun prog pre post ext env => (* Recapture cmp after rewriting *)
-                       match constr:(pre, post) with
-                       | ([[`?k <~~ ?cmp as _]] :: ?tenv, [[`?k <~~ ?cmp' as _]] :: ?tenv) => compile_simple_in_place_internal env cmp cmp' tenv ext
-                       end).
-
-Ltac compile_do_unwrap_W val :=
-  progress repeat match goal with
-  | [ H: WrapComp_W _ ↝ val |- _ ] =>
-    let eqn := fresh in
-    destruct (WrapComp_W_computes_to H) as [? (? & eqn)];
-      rewrite eqn in *; clear eqn H
-  end.
-
-Ltac compile_do_unwrap type wrapper key cmp tail val :=
-  lazymatch type with
-  | W => compile_do_unwrap_W val
-  | _ => fail 1 "Don't know how to unwrap" type
-  end;
-  let wrapper_head := head_constant wrapper in
-  cbv beta iota delta [WrappedCons wrapper_head].
-
-
 Ltac compile_do_use_transitivity_to_handle_head_separately :=
-  (* FIXME this is a very risky rule; it causes plenty of problems in particular
-     when a compilation step modifies two things at the same time. It should
-     probably be replaced by a bunch of specialized versions of this rule,
-     compiled with each lemma that handles the head. *)
-  (* There's an example of such a specialized lemma as CompileConstant in
-     Examples.v *)
+  (* NOTE: this is a very risky rule; it doesn't make much sense to apply it
+     unless one has a good way to handle the first goal that it produces. *)
   match_ProgOk ltac:(fun prog pre post ext env =>
                        match constr:(post) with
                        | Cons ?k _ _ =>
@@ -87,10 +31,93 @@ Ltac compile_do_extend_scalar_lifetime :=
                          end
                        end).
 
+(* Ltac case_unifiable x y when_unifiable unless_unifiable := *)
+(*   match goal with *)
+(*   | _ => let pr := constr:(eq_refl x : x = y) in first [ when_unifiable | fail 1 ] *)
+(*   | _ => unless_unifiable *)
+(*   end. *)
+
+Ltac strip_useless_binder tenv :=
+  match constr:(tenv) with
+  | (fun _ => ?tenv) => let tenv := strip_useless_binder tenv in constr:(tenv)
+  | _ => constr:(tenv)
+  end.
+
+Ltac call_tactic_after_moving_head_binding_to_separate_goal continuation :=
+  match_ProgOk
+    ltac:(fun prog pre post ext env =>
+            match constr:(pre, post) with
+            | (?tenv, Cons _ _ ?tenv') =>
+              let tenv' := strip_useless_binder tenv in
+              let pr := constr:(eq_refl tenv : tenv = tenv') in
+              first [ continuation | fail 1 ]
+            | _ => compile_do_use_transitivity_to_handle_head_separately; [ continuation | ]
+            end).
+
+(** The compile_simple* tactics handle simple gallina forms *)
+
+Hint Rewrite WrapComp_W_rewrite : compile_simple_db.
+
+Ltac compile_simple_internal env cmp ext :=
+  match cmp with
+  | ret (SCA ?av (?op ?lhs ?rhs)) => let facade_op := translate_op op in compile_binop av facade_op lhs rhs ext
+  | ret (@bool2val ?av (?op ?lhs ?rhs)) => let facade_op := translate_op op in compile_binop av facade_op lhs rhs ext
+  | ret (@bool2val ?av (@dec2bool _ _ (?op ?lhs ?rhs))) => let facade_op := translate_op op in compile_binop av facade_op lhs rhs ext
+  | ret (SCA _ ?w) => compile_constant w; compile_do_side_conditions
+  | ret (SCA ?av ?w) => compile_read (SCA av w) ext; compile_do_side_conditions
+  | ret (SCA ?av (?f ?w)) => compile_external_call_SCA av env f w ext
+  | (if ?t then ?tp else ?fp) => compile_if t tp fp
+  end.
+
+Ltac compile_simple_ProgOk prog pre post ext env :=
+  match constr:(pre, post) with
+  | (?tenv, Cons ?s ?cmp (fun _ => ?tenv)) => compile_simple_internal env cmp ext
+  end.
+
+Ltac compile_simple_same_tenv :=
+  autorewrite with compile_simple_db; (* Rewrite using user-provided lemmas *)
+  match_ProgOk compile_simple_ProgOk. (* Recapture cmp after rewriting *)
+
+Ltac compile_simple :=
+  debug "Compiling simple pattern";
+  call_tactic_after_moving_head_binding_to_separate_goal compile_simple_same_tenv.
+
+(** The compile_simple_inplce* tactic do roughly the same, but modifying an
+    existing binding: *)
+
+Ltac compile_simple_inplace_internal env cmp cmp' ext :=
+  match cmp' with
+  | (if ?t then ?tp else ?fp) => compile_if_in_place t tp fp
+  end.
+
+Ltac compile_simple_inplace_ProgOk prog pre post ext env :=
+  match constr:(pre, post) with
+  | (Cons ?s ?cmp ?tenv, Cons ?s ?cmp' ?tenv') => compile_simple_inplace_internal env cmp cmp' ext
+  end.
+
+Ltac compile_simple_inplace :=
+  debug "Compiling simple pattern in place";
+  autorewrite with compile_simple_db; (* Rewrite using user-provided lemmas *)
+  match_ProgOk compile_simple_inplace_ProgOk. (* Recapture cmp after rewriting *)
+
+Ltac compile_do_unwrap_W val :=
+  progress repeat match goal with
+  | [ H: WrapComp_W _ ↝ val |- _ ] =>
+    let eqn := fresh in
+    destruct (WrapComp_W_computes_to H) as [? (? & eqn)];
+      rewrite eqn in *; clear eqn H
+  end.
+
+Ltac compile_do_unwrap type wrapper key cmp tail val :=
+  lazymatch type with
+  | W => compile_do_unwrap_W val
+  | _ => fail 1 "Don't know how to unwrap" type
+  end;
+  let wrapper_head := head_constant wrapper in
+  cbv beta iota delta [WrappedCons wrapper_head].
+
 Ltac compile_do_cons :=
   debug "Moving head of Cons to separate goal";
-  (* match pre with *)
-  (* | context[key] =>  *)
   apply ProgOk_Transitivity_Cons.
 
 Ltac compile_do_chomp key :=
@@ -117,18 +144,36 @@ Ltac compile_skip :=
 (*! FIXME: The [ ... | fail] thing is needed: when removed the lazy match sometimes falls through *)
 Ltac compile_ProgOk p pre post ext env :=
   is_evar p;
-  lazymatch constr:(pre, post, ext) with
-  | (_,                           (@WrappedCons _ ?T ?wrapper ?k ?cmp ?tl) ?v, _) => first [compile_do_unwrap T wrapper k cmp tl v | fail ]
-  | (Cons ?k ?cmp _,              Cons ?k ?cmp _,                              _) => first [compile_do_chomp k | fail ]
-  | (Cons (Some ?k) ?cmp _,       Cons None ?cmp _,                            _) => first [compile_dealloc k cmp | fail ]
-  | (_,                           Cons None ?cmp ?tl,                          _) => first [compile_do_alloc cmp tl | fail ]
-  | (_,                           Cons ?k (Bind ?compA ?compB) ?tl,            _) => first [compile_do_bind k compA compB tl | fail ]
-  | (?tenv,                       Cons (Some ?k) ?cmp (fun _ => ?tenv),           _) => first [compile_simple k cmp | fail ]
-  | ([[`?k <~~ ?cmp as _]] :: ?tenv, [[`?k <~~ ?cmp' as _]] :: ?tenv,                _) => first [compile_simple_in_place k cmp cmp' | fail ]
-  | (?tenv,                       ?tenv,                                       _) => first [compile_skip | fail ]
+  lazymatch constr:(pre, post) with
+  (** Abstract manipulations **)
+  | (?tenv, ?tenv) => (* Empty program (side condition of a general lemma) *)
+    first [compile_skip | fail ]
+  | (Cons ?k ?cmp _, Cons ?k ?cmp _) => (* Chomp rule *)
+    first [compile_do_chomp k | fail ]
+  | (Cons (Some ?k) ?cmp _, Cons None ?cmp _) => (* Deallocation of head variable *)
+    first [compile_dealloc k cmp | fail ]
+  | (_, Cons None ?cmp ?tl) => (* Program does deallocation + something else; split *)
+    first [compile_do_alloc cmp tl | fail ]
+
+  (** Fiat manipulations **)
+  | (_, (@WrappedCons _ ?T ?wrap ?k ?cmp ?tl) ?v) => (* Wrapped constant *)
+    first [compile_do_unwrap T wrap k cmp tl v | fail ]
+  | (_, Cons ?k (Bind ?compA ?compB) ?tl) => (* Bindings *)
+    first [compile_do_bind k compA compB tl | fail ]
+
+  (** Concrete compilation **)
   | _ => match goal with
-        | _ => compile_do_extend_scalar_lifetime
-        | _ => compile_do_use_transitivity_to_handle_head_separately
+        | _ => (* Direct assignment *)
+          (lazymatch constr:(pre, post) with
+            | ([[`?k <~~ ?cmp as _]] :: ?tenv, [[`?k <~~ ?cmp' as _]] :: ?tenv') => (* In place modifications *)
+              first [ compile_simple_inplace | fail ]
+            | (?tenv, Cons (Some ?k) ?cmp ?tenv') => (* Assignments to new variables *)
+              first [ compile_simple | fail ]
+            end)
+        | _ => (* Fallback abstract manipulation *)
+          (match goal with
+           | _ => compile_do_extend_scalar_lifetime
+           end)
         end
   end.
 
@@ -139,11 +184,11 @@ Ltac is_pushable_head_constant f :=
   | _ => idtac
   end.
 
-Ltac compile_rewrite :=
-  match goal with
+Ltac compile_rewrite p pre post ext env :=
+  match post with
   (*! FIXME Why is setoid needed here? !*)
-  | [  |- appcontext[if ?b then ?x else ?y] ] => is_dec b; setoid_rewrite (dec2bool_correct b x y)
-  | [  |- appcontext[?f (if ?b then ?x else ?y)] ] => is_pushable_head_constant f; setoid_rewrite (push_if f x y b)
+  | appcontext[if ?b then ?x else ?y] => is_dec b; setoid_rewrite (dec2bool_correct b x y)
+  | appcontext[?f (if ?b then ?x else ?y)] => is_pushable_head_constant f; setoid_rewrite (push_if f x y b)
   end.
 
 Definition IsFacadeProgramImplementing {av} cmp env prog :=
@@ -167,9 +212,10 @@ Ltac compile_step_with worker :=
   idtac;
   match goal with
   | _ => start_compiling
-  | _ => compile_rewrite
   | _ => compile_do_side_conditions
+  | _ => match_ProgOk compile_rewrite
   | _ => match_ProgOk worker
+  | _ => progress (subst || intros)
   end.
 
 Ltac compile_step :=
